theories/datatypes_properties.v
@@ -370,27 +370,5 @@ Definition eqmemory_typeP : Equality.axiom memory_type_eqb :=
 Canonical Structure memory_type_eqMixin := EqMixin eqmemory_typeP.
 Canonical Structure memory_type_eqType := Eval hnf in EqType memory_type memory_type_eqMixin.
 
-Scheme Equality for res_crash.
-Definition res_crash_eqb c1 c2 := is_left (res_crash_eq_dec c1 c2).
-Definition eqres_crashP : Equality.axiom res_crash_eqb :=
-  eq_dec_Equality_axiom res_crash_eq_dec.
-
-Canonical Structure res_crash_eqMixin := EqMixin eqres_crashP.
-Canonical Structure res_crash_eqType := Eval hnf in EqType res_crash res_crash_eqMixin.
-
-Definition res_step_eq_dec : forall r1 r2 : res_step, {r1 = r2} + {r1 <> r2}.
-Proof.
-  (decidable_equality_step;
-    last by apply: (eq_comparable (_ : seq administrative_instruction)));
-    decidable_equality.
-Defined.
-
-Definition res_step_eqb (r1 r2 : res_step) : bool := res_step_eq_dec r1 r2.
-Definition eqres_stepP : Equality.axiom res_step_eqb :=
-  eq_dec_Equality_axiom res_step_eq_dec.
-
-Canonical Structure res_step_eqMixin := EqMixin eqres_stepP.
-Canonical Structure res_step_eqType := Eval hnf in EqType res_step res_step_eqMixin.
-
 End Host.
 
