theories/instantiation_func.v
@@ -1,0 +1,346 @@
+From mathcomp Require Import ssreflect ssrbool ssrnat eqtype seq.
+From Wasm Require Import opsem interpreter_func instantiation_spec.
+From Coq Require Import BinNat.
+
+Section Instantiation_func.
+
+Import EmptyHost.
+Import Interpreter_func.
+
+Let alloc_funcs := alloc_funcs host_function_eqType.
+Let alloc_tabs := alloc_tabs host_function_eqType.
+Let alloc_mems := alloc_mems host_function_eqType.
+Let alloc_globs := alloc_globs host_function_eqType.
+Let check_bounds_elem := check_bounds_elem host_function_eqType.
+Let check_bounds_data := check_bounds_data host_function_eqType.
+Let init_tabs := init_tabs host_function_eqType.
+Let init_mems := init_mems host_function_eqType.
+
+Let instantiate := instantiate host_function_eqType host_instance.
+
+Let run_v := run_v tt.
+
+
+Definition gather_m_f_type (tfs : list function_type) (m_f : module_func) : option function_type :=
+  let '(Mk_typeidx i) := m_f.(modfunc_type) in
+  if i < List.length tfs then List.nth_error tfs i
+  else None.
+
+Definition gather_m_f_types (tfs : list function_type) (m_fs : list module_func) : option (list function_type) :=
+  list_extra.those (List.map (gather_m_f_type tfs) m_fs).
+
+Definition module_import_typer (tfs : list function_type) (imp : import_desc) : option extern_t :=
+  match imp with
+  | ID_func i =>
+    if i < List.length tfs then
+      match List.nth_error tfs i with
+      | None => None
+      | Some ft => Some (ET_func ft)
+      end
+    else None
+  | ID_table t_t =>
+    if module_tab_typing {| modtab_type := t_t |} then Some (ET_tab t_t) else None
+  | ID_mem mt =>
+    if module_mem_typing mt then Some (ET_mem mt) else None
+  | ID_global gt => Some (ET_glob gt)
+  end.
+
+Definition module_imports_typer (tfs : list function_type) (imps : list module_import) : option (list extern_t) :=
+  those (List.map (fun imp => module_import_typer tfs imp.(imp_desc)) imps).
+
+Definition module_export_typer (c : t_context) (exp : module_export_desc) : option extern_t :=
+  match exp with
+  | MED_func (Mk_funcidx i) =>
+    if i < List.length c.(tc_func_t) then
+      match List.nth_error c.(tc_func_t) i with
+      | None => None
+      | Some ft => Some (ET_func ft)
+      end
+    else None
+  | MED_table (Mk_tableidx i) =>
+    if i < List.length c.(tc_table) then
+      match List.nth_error c.(tc_table) i with
+      | None => None
+      | Some t_t => Some (ET_tab t_t)
+      end
+    else None
+  | MED_mem (Mk_memidx i) =>
+    if i < List.length c.(tc_memory) then
+      match List.nth_error c.(tc_memory) i with
+      | None => None
+      | Some lim => Some (ET_mem lim)
+      end
+    else None
+  | MED_global (Mk_globalidx i) =>
+    if i < List.length c.(tc_global) then
+      match List.nth_error c.(tc_global) i with
+      | None => None
+      | Some g => Some (ET_glob g)
+      end
+    else None
+  end.
+
+Definition module_exports_typer (c : t_context) exps :=
+  those (List.map (fun exp => module_export_typer c exp.(modexp_desc)) exps).
+
+Definition gather_m_g_types (mgs : list module_glob) : list global_type :=
+  List.map (fun mg => mg.(modglob_type)) mgs.
+
+Definition module_func_type_checker (c : t_context) (m : module_func) : bool :=
+  let '{| modfunc_type := Mk_typeidx i; modfunc_locals := t_locs; modfunc_body := b_es |} := m in
+  (i < List.length c.(tc_types_t)) &&
+  match List.nth_error c.(tc_types_t) i with
+  | None => false
+  | Some (Tf tn tm) =>
+    let c' := {|
+      tc_types_t := c.(tc_types_t);
+      tc_func_t := c.(tc_func_t);
+      tc_global := c.(tc_global);
+      tc_table := c.(tc_table);
+      tc_memory := c.(tc_memory);
+      tc_local := List.app c.(tc_local) (List.app tn t_locs);
+      tc_label := tm :: c.(tc_label);
+      tc_return := Some tm;
+    |} in
+    type_checker.b_e_type_checker c' b_es (Tf [::] tm)
+  end.
+
+Definition module_tab_type_checker := module_tab_typing.
+Definition module_memory_type_checker := module_mem_typing.
+
+Definition module_glob_type_checker (c : t_context) (mg : module_glob) : bool :=
+  let '{| modglob_type := tg; modglob_init := es |} := mg in
+  const_exprs c es &&
+  type_checker.b_e_type_checker c es (Tf nil [::tg.(tg_t)]).
+
+Definition module_elem_type_checker (c : t_context) (e : module_element) : bool :=
+  let '{| modelem_table := Mk_tableidx t; modelem_offset := es; modelem_init := is_ |} := e in
+  const_exprs c es &&
+  type_checker.b_e_type_checker c es (Tf nil [::T_i32]) &&
+  (t < List.length c.(tc_table)) &&
+  seq.all (fun '(Mk_funcidx i) => i < List.length c.(tc_func_t)) is_.
+
+Definition module_data_type_checker (c : t_context) (d : module_data) : bool :=
+  let '{| moddata_data := Mk_memidx d; moddata_offset := es; moddata_init := bs |} := d in
+  const_exprs c es &&
+  type_checker.b_e_type_checker c es (Tf nil [::T_i32]) &&
+  (d < List.length c.(tc_memory)).
+
+Definition module_start_type_checker (c : t_context) (ms : module_start) : bool :=
+  module_start_typing c ms.
+
+Definition module_type_checker (m : module) : option ((list extern_t) * (list extern_t)) :=
+  let '{|
+    mod_types := tfs;
+    mod_funcs := fs;
+    mod_tables := ts;
+    mod_mems := ms;
+    mod_globals := gs;
+    mod_elem := els;
+    mod_data := ds;
+    mod_start := i_opt;
+    mod_imports := imps;
+    mod_exports := exps;
+    |} := m in
+  match (gather_m_f_types tfs fs, module_imports_typer tfs imps) with
+  | (Some fts, Some impts) =>
+    let ifts := ext_t_funcs impts in
+    let its := ext_t_tabs impts in
+    let ims := ext_t_mems impts in
+    let igs := ext_t_globs impts in
+    let gts := gather_m_g_types gs in
+    let c := {|
+      tc_types_t := tfs;
+      tc_func_t := List.app ifts fts;
+      tc_global := List.app igs gts;
+      tc_table := List.app its (List.map (fun t => t.(modtab_type)) ts);
+      tc_memory := List.app ims ms;
+      tc_local := nil;
+      tc_label := nil;
+      tc_return := None |} in
+    let c' := {|
+      tc_types_t := nil;
+      tc_func_t := nil;
+      tc_global := igs;
+      tc_table := nil;
+      tc_memory := nil;
+      tc_local := nil;
+      tc_label := nil;
+      tc_return := None
+    |} in
+    if seq.all (module_func_type_checker c) fs &&
+       seq.all module_tab_type_checker ts &&
+       seq.all module_memory_type_checker ms &&
+       seq.all (module_glob_type_checker c') gs &&
+       seq.all (module_elem_type_checker c) els &&
+       seq.all (module_data_type_checker c) ds &&
+       pred_option (module_start_type_checker c) i_opt then
+       match module_exports_typer c exps with
+       | Some expts => Some (impts, expts)
+       | None => None
+       end
+    else None
+  | (Some _, None) | (None, Some _) | (None, None) => None
+  end.
+
+Definition external_type_checker (s : store_record) (v : v_ext) (e : extern_t) : bool :=
+  match (v, e) with
+  | (MED_func (Mk_funcidx i), ET_func tf) =>
+    (i < List.length s.(s_funcs)) &&
+    match List.nth_error s.(s_funcs) i with
+    | None => false
+    | Some cl => tf == operations.cl_type cl
+    end
+  | (MED_table (Mk_tableidx i), ET_tab tf) =>
+(* TODO   let '{| tt_limits := lim; tt_elem_type := elem_type_tt |} := tf in*)
+    (i < List.length s.(s_tables)) &&
+    match List.nth_error s.(s_tables) i with
+    | None => false
+    | Some ti => typing.tab_typing ti tf
+    end
+  | (MED_mem (Mk_memidx i), ET_mem mt) =>
+    (i < List.length s.(s_mems)) &&
+    match List.nth_error s.(s_mems) i with
+    | None => false
+    | Some m => typing.mem_typing m mt
+    end
+  | (MED_global (Mk_globalidx i), ET_glob gt) =>
+    (i < List.length s.(s_globals)) &&
+    match List.nth_error s.(s_globals) i with
+    | None => false
+    | Some g => typing.global_agree g gt
+    end
+  | (_, _) => false
+  end.
+
+Definition interp_get_v (s : store_record) (inst : instance) (b_es : list basic_instruction) : option value (* TODO: isa mismatch *) :=
+  match run_v s (Build_frame [::] inst) (operations.to_e_list b_es) 2 with
+  | (_, interpreter_func.R_value vs) =>
+    match vs with
+    | [:: v] => Some v
+    | _ => None
+    end
+  | _ => None
+  end.
+
+Definition interp_get_i32 (s : store_record) (inst : instance) (b_es : list basic_instruction) : option i32 (* TODO: isa mismatch *) :=
+  match interp_get_v s inst b_es with
+  | Some (VAL_int32 c) => Some c
+  | _ => None
+  end.
+
+Definition interp_alloc_module (s : store_record) (m : module) (imps : list v_ext) (gvs : list value) : (store_record * instance * list module_export) :=
+  let i_fs := List.map (fun i => Mk_funcidx i) (seq.iota (List.length s.(s_funcs)) (List.length m.(mod_funcs))) in
+  let i_ts := List.map (fun i => Mk_tableidx i) (seq.iota (List.length s.(s_tables)) (List.length m.(mod_tables))) in
+  let i_ms := List.map (fun i => Mk_memidx i) (seq.iota (List.length s.(s_mems)) (List.length m.(mod_mems))) in
+  let i_gs := List.map (fun i => Mk_globalidx i) (seq.iota (List.length s.(s_globals)) (min (List.length m.(mod_globals)) (List.length gvs))) in
+  let inst := {|
+    inst_types := m.(mod_types);
+    inst_funcs := List.map (fun '(Mk_funcidx i) => i) (List.app (ext_funcs imps) i_fs);
+    inst_tab := List.map (fun '(Mk_tableidx i) => i) (List.app (ext_tabs imps) i_ts);
+    inst_memory := List.map (fun '(Mk_memidx i) => i) (List.app (ext_mems imps) i_ms);
+    inst_globs := List.map (fun '(Mk_globalidx i) => i) (List.app (ext_globs imps) i_gs);
+  |} in
+  let '(s1, _) := alloc_funcs s m.(mod_funcs) inst in
+  let '(s2, _) := alloc_tabs s1 (List.map (fun t => t.(modtab_type)) m.(mod_tables)) in
+  let '(s3, _) := alloc_mems s2 m.(mod_mems) in
+  let '(s', _) := alloc_globs s3 m.(mod_globals) gvs in
+  let exps := List.map (fun m_exp => {| modexp_name := m_exp.(modexp_name); modexp_desc := export_get_v_ext inst m_exp.(modexp_desc) |}) m.(mod_exports) in
+  (s', inst, exps).
+
+Definition interp_instantiate (hs : host_state) (s : store_record) (m : module) (v_imps : list v_ext) : option ((host_state * store_record * instance * list module_export) * option nat) :=
+  match module_type_checker m with
+  | None => None
+  | Some (t_imps, t_exps) =>
+    if seq.all2 (external_type_checker s) v_imps t_imps then
+      let g_inits_opt :=
+        let c := {|
+          inst_types := nil;
+          inst_funcs := nil;
+          inst_tab := nil;
+          inst_memory := nil;
+          inst_globs := List.map (fun '(Mk_globalidx i) => i) (ext_globs v_imps);
+        |} in
+        those (map (fun g => interp_get_v s c g.(modglob_init)) m.(mod_globals)) in
+      match g_inits_opt with
+      | None => None
+      | Some g_inits =>
+        let '(s', inst, v_exps) := interp_alloc_module s m v_imps g_inits in
+        let e_offs_opt := those (map (fun e => interp_get_i32 s' inst e.(modelem_offset)) m.(mod_elem)) in
+        match e_offs_opt with
+        | None => None
+        | Some e_offs =>
+          let d_offs_opt := those (map (fun d => interp_get_i32 s' inst d.(moddata_offset)) m.(mod_data)) in
+          match d_offs_opt with
+          | None => None
+          | Some d_offs =>
+            if check_bounds_elem inst s' m e_offs &&
+               check_bounds_data inst s' m d_offs then
+              let start : option nat := operations.option_bind (fun i_s => List.nth_error inst.(inst_funcs) (match i_s.(modstart_func) with Mk_funcidx i => i end)) m.(mod_start) in
+              let s'' := init_tabs s' inst (List.map nat_of_int e_offs) m.(mod_elem) in
+              let s_end := init_mems s'' inst (List.map N_of_int d_offs) m.(mod_data) in
+              Some ((hs, s_end, inst, v_exps), start)
+            else None
+          end
+        end
+      end
+    else None
+  end.
+
+Lemma interp_instantiate_imp_instantiate :
+  forall (hs : host_state) s m v_imps hs s_end inst v_exps start,
+  interp_instantiate hs s m v_imps = Some ((hs, s_end, inst, v_exps), start) ->
+  instantiate s m v_imps ((s_end, inst, v_exps), start).
+Proof.
+Admitted. (* TODO *)
+
+Definition empty_store_record : store_record := {|
+    s_funcs := nil;
+    s_tables := nil;
+    s_mems := nil;
+    s_globals := nil;
+  |}.
+
+Definition interp_instantiate_wrapper (m : module) : option ((host_state * store_record * instance * list module_export) * option nat) :=
+  interp_instantiate tt empty_store_record m nil.
+
+Definition lookup_exported_function (n : name) (store_inst_exps : host_state * store_record * instance * list module_export)
+    : option (host_state * store_record * frame * seq administrative_instruction) :=
+  let '(hs, s, inst, exps) := store_inst_exps in
+  List.fold_left
+    (fun acc e =>
+      match acc with
+      | Some cfg => Some cfg
+      | None =>
+        if e.(modexp_name) == n then
+          match e.(modexp_desc) with
+          | MED_func (Mk_funcidx fi) =>
+(*            Some (s, (Build_frame nil inst), [::AI_invoke fi])*)
+            match List.nth_error s.(s_funcs) fi with
+            | None => None
+            | Some fc => Some (hs, s, (Build_frame nil inst), [::AI_invoke fi])
+            end
+          | _ => None
+          end
+        else None
+      end)
+    exps
+    None.
+
+End Instantiation_func.
+
+Module Instantiation.
+
+Import EmptyHost.
+
+Definition lookup_exported_function :
+    name -> host_state * store_record * instance * seq module_export ->
+    option (host_state * store_record * frame * seq administrative_instruction) :=
+  lookup_exported_function.
+
+Definition interp_instantiate_wrapper :
+  module ->
+  option (host_state * store_record * instance * seq module_export * option nat) :=
+  interp_instantiate_wrapper.
+
+End Instantiation.
