theories/interpreter_func.v
@@ -3113,4 +3113,3 @@ Definition is_const_list : list administrative_instruction -> option (list value
   @those_const_list.
 
 End Interpreter_func.
-
